projection/proofs/bakery_to_endpointProofScript.sml
@@ -1,8 +1,215 @@
-open preamble endpointLangTheory bakery_to_endpoint
-              endpointSemanticsTheory;
+open preamble endpointLangTheory bakery_to_endpointTheory
+              endpointSemanticsTheory endpointPropsTheory
+              semBakeryTheory;
 
 val _ = new_theory "bakery_to_endpointProof";
 
 
+val all_distinct_nub' = Q.store_thm("all_distinct_nub'",
+  `∀l. ALL_DISTINCT (nub' l)`,
+  rw [ALL_DISTINCT,nub'_def]
+  \\ Induct_on `l`
+  \\ rw [ALL_DISTINCT,nub'_def,FILTER_ALL_DISTINCT,MEM_FILTER]
+);
+
+val procsOf_all_distinct = Q.store_thm("procsOf_all_distinct",
+  `∀c. ALL_DISTINCT (procsOf c)`,
+  Induct_on `c` >> rw [procsOf_def,ALL_DISTINCT,all_distinct_nub']
+);
+
+val cn_ignore_com = Q.store_thm("cn_ignore_com",
+  `∀p1 v1 p2 v2 s c' pl q.
+    ¬MEM p1 pl ∧ ¬MEM p2 pl
+    ⇒ compile_network s (Com p1 v1 p2 v2 c') pl q = compile_network s c' pl q`,
+  Induct_on `pl`
+  \\ rw [compile_network_def,project_def,projectS_def]
+);
+
+val cn_ignore_sel = Q.store_thm("cn_ignore_sel",
+  `∀p1 b p2 s c' pl q.
+    ¬MEM p1 pl ∧ ¬MEM p2 pl
+    ⇒ compile_network s (Sel p1 b p2 c') pl q = compile_network s c' pl q`,
+  Induct_on `pl`
+  \\ rw [ compile_network_def,project_def,projectS_def
+        , projectQ_def,FLOOKUP_UPDATE]
+);
+
+val cn_ignore_let = Q.store_thm("cn_ignore_let",
+  `∀p s v f vl c pl q.
+    ¬MEM p pl
+    ⇒ compile_network s (Let v p f vl c) pl q = compile_network s c pl q`,
+  Induct_on `pl`
+  \\ rw [ compile_network_def,project_def,projectS_def
+        , projectQ_def,FLOOKUP_UPDATE]
+);
+
+val cn_ignore_queue_update = Q.store_thm("cn_ignore_queue_update",
+  `∀p s c pl q q'.
+    ¬MEM p pl
+    ⇒ compile_network s c pl (q |+ (p,q')) = compile_network s c pl q`,
+  Induct_on `pl`
+  \\ rw [ compile_network_def,project_def,projectS_def
+        , projectQ_def,FLOOKUP_UPDATE]
+);
+
+val cn_ignore_state_update = Q.store_thm("cn_ignore_state_update",
+  `∀p v d s c pl q.
+    ¬MEM p pl
+    ⇒ compile_network (s |+ ((v,p),d)) c pl q = compile_network s c pl q`,
+  Induct_on `pl`
+  \\ rw [ compile_network_def,project_def,projectS_def
+        , projectQ_def,FLOOKUP_UPDATE]
+);
+
+val RTC_TRANS = save_thm ("RTC_TRANS",
+  RTC_RULES |> CONV_RULE FORALL_AND_CONV |> CONJUNCTS |> el 2);
+
+
+(* Move to endpointPropsTheory *)
+val trans_dequeue_gen = Q.store_thm("trans_dequeue_gen",
+  `∀d s s' v p1 p2 e q1 q2.
+    s.queue = q1 ⧺ [(p1,d)] ⧺ q2
+    ∧ p1 ≠ p2 ∧ EVERY (λ(p,_). p ≠ p1) q1
+    ∧ s' = s with <|queue := q1 ⧺ q2; bindings := s.bindings |+ (v,d)|>
+    ⇒ trans (NEndpoint p2 s (Receive p1 v e))
+            LTau
+            (NEndpoint p2 s' e)`,
+  rw [] >> drule trans_dequeue >> rw []
+);
+
+val trans_enqueue_choice_gen = Q.store_thm("trans_enqueue_choice_gen",
+  `∀s p1 p2 e s' b.
+    p1 ≠ p2
+    ∧ s' = s with queue := SNOC (p1,if b then [1w] else [0w]) s.queue
+    ⇒ trans (NEndpoint p2 s e)
+            (LExtChoice p1 b p2)
+            (NEndpoint p2 s' e)`,
+  rw []
+  >- (drule trans_enqueue_choice_l >> rw [])
+  >- (drule trans_enqueue_choice_r >> rw [])
+);
+
+val trans_let_gen = Q.store_thm("trans_let_gen",
+  `∀s s' v p f vl e.
+    EVERY IS_SOME (MAP (FLOOKUP s.bindings) vl)
+    ∧ s' = (s with bindings := s.bindings |+ (v,f(MAP (THE o FLOOKUP s.bindings) vl)))
+    ⇒ trans (NEndpoint p s (Let v f vl e))
+             LTau
+             (NEndpoint p s' e)`,
+  rw [endpointSemanticsTheory.trans_let]
+);
+
+val compile_network_preservation = Q.store_thm("compile_network_preservation"
+  `∀s c α τ s' c'. trans (s,c) (α,τ) (s',c')
+    ⇒ ∃q. reduction^* (compile_network s  c  (procsOf c) FEMPTY)
+                      (compile_network s' c' (procsOf c) q)`,
+  ho_match_mp_tac trans_pairind
+  \\ rw [ compile_network_def
+        , procsOf_def
+        , procsOf_all_distinct
+        , nub'_def
+        , reduction_def
+        , project_def
+        , FILTER_FILTER
+        , FOLDL
+        , fupdate_projectS]
+  (* Com *)
+  >- (Q.EXISTS_TAC `FEMPTY`
+     \\ IMP_RES_TAC lookup_projectS
+     \\ rw [projectQ_def]
+     \\ MAP_EVERY Q.ABBREV_TAC [ `l = FILTER (λy. p1 ≠ y ∧ p2 ≠ y) (nub' (procsOf c'))`
+                               , `s'   = s |+ ((v2,p2),d)`
+                               , `s1   = projectS p1 s`
+                               , `s2   = projectS p2 s`
+                               , `s2'  = projectS p2 s'`
+                               , `cp1  = project p1 c'`
+                               , `cp2  = project p2 c'`
+                               , `ns   = compile_network s' c' l FEMPTY`
+                               , `s1q  = <|bindings := s1; queue := []|>`
+                               , `s2q  = <|bindings := s2; queue := []|>`
+                               ]
+     \\ `compile_network s (Com p1 v1 p2 v2 c') l FEMPTY = ns`
+        by (rw [Abbr `l`, Abbr `ns`, Abbr `s'`, MEM_FILTER
+               , cn_ignore_com, cn_ignore_state_update])
+     \\ ASM_REWRITE_TAC []
+     \\ pop_assum (K ALL_TAC)
+     \\ ho_match_mp_tac RTC_TRANS
+     \\ Q.EXISTS_TAC
+        `NPar  (NEndpoint p1 s1q cp1)
+        (NPar  (NEndpoint p2 (s2q with queue := SNOC (p1,d) s2q.queue)
+                             (Receive p1 v2 cp2)) ns)`
+     \\ rw [reduction_def]
+     >- (ho_match_mp_tac trans_com_l
+        \\ MAP_EVERY Q.EXISTS_TAC [`p1`,`p2`,`d`]
+        \\ rw []
+        >- (ho_match_mp_tac trans_send
+           \\ rw [Abbr `s1q`])
+        >- (ho_match_mp_tac trans_par_l
+           \\ ho_match_mp_tac trans_enqueue
+           \\ rw []))
+     >- (ho_match_mp_tac RTC_SINGLE
+        \\ rw [reduction_def]
+        \\ ho_match_mp_tac trans_par_r
+        \\ ho_match_mp_tac trans_par_l
+        \\ ho_match_mp_tac trans_dequeue_gen
+        \\ MAP_EVERY Q.EXISTS_TAC [`d`,`[]`,`[]`]
+        \\ rw [Abbr `s2q`, Abbr `s2`,Abbr `s'`,Abbr `s2'`,projectS_fupdate]))
+  (* Sel *)
+  >- (Q.EXISTS_TAC `FEMPTY |+ (p2,[(p1,if b then [1w] else [0w])])`
+      \\ fs [projectQ_def,FLOOKUP_UPDATE]
+      \\ MAP_EVERY Q.ABBREV_TAC [ `l  = FILTER (λy. p1 ≠ y ∧ p2 ≠ y) (nub' (procsOf c'))`
+                                , `s1   = projectS p1 s`
+                                , `s2   = projectS p2 s`
+                                , `cp1  = project p1 c'`
+                                , `cp2  = project p2 c'`
+                                , `ns   = compile_network s c' l FEMPTY`
+                                ]
+      \\ `compile_network s (Sel p1 b p2 c') l FEMPTY = ns`
+         by (rw [Abbr `l`, Abbr `ns`, MEM_FILTER, cn_ignore_sel])
+      \\ `compile_network s c' l
+              (FEMPTY |+ (p2,[(p1,if b then [1w] else [0w])])) = ns`
+          by (rw [Abbr `l`, Abbr `ns`, MEM_FILTER, cn_ignore_queue_update])
+      \\ fs []
+      \\ pop_assum (K ALL_TAC)
+      \\ pop_assum (K ALL_TAC)
+      \\ ho_match_mp_tac RTC_SINGLE
+      \\ fs [reduction_def]
+      \\ ho_match_mp_tac trans_com_choice_l
+      \\ MAP_EVERY Q.EXISTS_TAC [`p1`,`p2`,`b`]
+      \\ fs []
+      \\ CONJ_TAC
+      >- (ho_match_mp_tac trans_int_choice >> rw [])
+      >- (ho_match_mp_tac trans_par_l
+         \\ ho_match_mp_tac trans_enqueue_choice_gen
+         \\ rw []))
+  (* Let *)
+  >- (Q.EXISTS_TAC `FEMPTY`
+     \\ fs [projectQ_def,FLOOKUP_UPDATE]
+     \\ MAP_EVERY Q.ABBREV_TAC [ `l  = FILTER (λy. p ≠ y) (nub' (procsOf c'))`
+                               , `s' = s |+ ((v,p),f (MAP (THE ∘ FLOOKUP s) (MAP (λv. (v,p)) vl)))`
+                               , `s1   = projectS p s`
+                               , `s1'  = projectS p s'`
+                               , `cp1  = project p c'`
+                               , `cp2  = project p c'`
+                               , `ns   = compile_network s' c' l FEMPTY`
+                               , `sq  = <|bindings := s1; queue := []|>`
+                               , `sq'  = <|bindings := s1'; queue := []|>`
+                               ]
+     \\`compile_network s (Let v p f vl c') l FEMPTY = ns`
+     by (rw [ Abbr `l`, Abbr `ns`, Abbr `s'`, MEM_FILTER
+            , cn_ignore_let , cn_ignore_state_update])
+     \\ ASM_REWRITE_TAC []
+     \\ pop_assum (K ALL_TAC)
+     \\ ho_match_mp_tac RTC_SINGLE
+     \\ rw [reduction_def]
+     \\ ho_match_mp_tac trans_par_l
+     \\ ho_match_mp_tac trans_let_gen
+     \\ UNABBREV_ALL_TAC
+     \\ rw []
+     >- (Induct_on `vl` \\ rw [lookup_projectS'])
+     >- (rw [projectS_fupdate] >> rpt AP_TERM_TAC
+        \\ Induct_on `vl` >> rw [lookup_projectS']))
+  \\ cheat
+);
 
 val _ = export_theory ()
